src/SDK/MessageBody.dfy
@@ -174,6 +174,8 @@ module MessageBody {
     ensures match result
       case Failure(e) => true
       case Success(resultSuccess) => exists frames: seq<Frame> | ValidFrames(frames) ::
+        && |frames| < UINT32_LIMIT
+        && (forall frame: Frame | frame in frames :: frame.Valid())
         && FramesToSequence(frames) == resultSuccess
         && FramesEncryptPlaintext(frames, plaintext)
   { 
